finishing funcD and noting the first issue with expr.

MirrorCharge!/src/ILogicFunc.v
@@ -5,109 +5,261 @@ Require Import MapPositive.
 Definition logic_index := positive.
 Definition ref_index := positive.
 
-Inductive typ := 
-	| tyPred : logic_index -> typ
-	| tyRef    : ref_index -> typ
-	| tyArr  : typ -> typ -> typ.
-	
+Inductive typ :=
+| tyPred : logic_index -> typ
+| tyRef    : ref_index -> typ
+| tyArr  : typ -> typ -> typ.
+
 Section TypeDenotation.
 
-	Definition var_logic_map := PositiveMap.t ({x : Type & ILogicOps x}).
-	Definition ref_type_map := PositiveMap.t Type.
-	
-	Fixpoint typD (vlm : var_logic_map) (rtm : ref_type_map) (l : list Type) (t : typ) :=
-		match t with
-			| tyPred p => match PositiveMap.find p vlm with
-						      | Some T => projT1 T
-						      | None => Empty_set
-						  end
-			| tyRef p => match PositiveMap.find p rtm with
-						      | Some T => T
-						      | None => Empty_set
-						  end
-			| tyArr t1 t2 => typD vlm rtm l t1 -> typD vlm rtm l t2
-		end.			  
+  Definition var_logic_map := PositiveMap.t {x : Type & ILogicOps x}.
+  Definition ref_type_map := PositiveMap.t Type.
+
+  Fixpoint typD (vlm : var_logic_map) (rtm : ref_type_map) (l : list Type) (t : typ) :=
+    match t with
+      | tyPred p =>
+        match PositiveMap.find p vlm with
+	  | Some T => projT1 T
+	  | None => Empty_set
+	end
+      | tyRef p =>
+        match PositiveMap.find p rtm with
+	  | Some T => T
+	  | None => Empty_set
+	end
+      | tyArr t1 t2 => typD vlm rtm l t1 -> typD vlm rtm l t2
+    end.
 
 End TypeDenotation.
 
 Inductive ilfunc :=
-	| ilf_true : logic_index -> ilfunc
-	| ilf_false : logic_index -> ilfunc
-	| ilf_and : logic_index -> ilfunc
-	| ilf_or: logic_index -> ilfunc
-	| ilf_impl : logic_index -> ilfunc
-	| fref (fi : positive).
-	 
+| ilf_true : logic_index -> ilfunc
+| ilf_false : logic_index -> ilfunc
+| ilf_and : logic_index -> ilfunc
+| ilf_or: logic_index -> ilfunc
+| ilf_impl : logic_index -> ilfunc
+| fref (fi : positive).
+
 Section RFunc.
   Variable ts : var_logic_map.
   Variable rs : ref_type_map.
-  
+
   Record function := F
   { ftype : typ
   ; fdenote : typD ts rs nil ftype
   }.
-  
-  Definition fun_logic_map := PositiveMap.t function.  
-  
-  Variable fs : fun_logic_map.
-  
+
+  Definition fun_map := PositiveMap.t function.
+
+  Variable fs : fun_map.
+
   Definition typeof_func (f : ilfunc) : option typ :=
-  	match f with
-  		| ilf_true i
-  		| ilf_false i => match PositiveMap.find i ts with
-  							| Some _ => Some (tyPred i)
-  							| None => None
-  						 end
-  		| ilf_and i 
-  		| ilf_or i 
-  		| ilf_impl i => match PositiveMap.find i ts with
-  							| Some _ => Some (tyArr (tyPred i) (tyArr (tyPred i) (tyPred i)))
-  							| None => None
-  						end
-  		| fref i => match PositiveMap.find i fs with
-  				    | Some f => Some (ftype f)
-  				    | None => None
-  				    end
-  	end.
-  Print RFunc.
-  	
-  	Definition funcD : forall f : ilfunc,
-            match typeof_func f with
-            | Some t => typD ts rs nil t
-            | None => unit
-            end.
-    intros f.
-    refine (match f as f return (match typeof_func f with
-									| Some t => typD ts rs nil t
-									| None => unit
-									end) with 
-			| ilf_true i => 
-			  match PositiveMap.find i ts as x
-			    return x = PositiveMap.find i ts ->
-			           (match match x with
-			                    | Some _ => Some (tyPred i)
-			                    | None => None
-			                  end
-			            with
-			              | Some t => typD ts rs nil t
-			              | None => unit
-			            end)
-			   with			
-  				| Some t => fun pf => match pf in _ = t return 
-  				match t with
-| Some T => projT1 T
-| None => Empty_set
-end with
-  				                      | eq_refl => @ltrue _ (projT2 t)
-  				                      end
-  			    | None => fun _ => tt
-  			   end eq_refl
-			| _ => _ 
-			end).
-			simpl.
-  
-  
-  Definition val : function := F (tvArr tvProp tvProp) not. 
-  
-Section oneuthoe.
-Context {A : Type} `{HIL : ILogic A}.
+    match f with
+      | ilf_true i
+      | ilf_false i =>
+        match PositiveMap.find i ts with
+  	  | Some _ => Some (tyPred i)
+  	  | None => None
+  	end
+      | ilf_and i
+      | ilf_or i
+      | ilf_impl i =>
+        match PositiveMap.find i ts with
+  	  | Some _ => Some (tyArr (tyPred i) (tyArr (tyPred i) (tyPred i)))
+  	  | None => None
+  	end
+      | fref i =>
+        match PositiveMap.find i fs with
+  	  | Some f => Some (ftype f)
+  	  | None => None
+  	end
+    end.
+
+  Definition funcD (f : ilfunc) :
+    match typeof_func f with
+      | Some t => typD ts rs nil t
+      | None => unit
+    end :=
+    match f as f return match typeof_func f with
+			  | Some t => typD ts rs nil t
+			  | None => unit
+			end with
+      | ilf_true i =>
+	match PositiveMap.find i ts as x
+	      return x = PositiveMap.find i ts ->
+		     (match match x with
+			      | Some _ => Some (tyPred i)
+			      | None => None
+			    end
+		      with
+			| Some t => typD ts rs nil t
+			| None => unit
+		      end)
+	with
+  	  | Some t => fun pf => match pf in _ = t return
+  				      match t with
+                                        | Some T => projT1 T
+                                        | None => Empty_set
+                                      end with
+  				  | eq_refl => @ltrue _ (projT2 t)
+  				end
+  	  | None => fun _ => tt
+  	end eq_refl
+      | ilf_false i =>
+	match PositiveMap.find i ts as x
+	      return x = PositiveMap.find i ts ->
+		     (match match x with
+			      | Some _ => Some (tyPred i)
+			      | None => None
+			    end
+		      with
+			| Some t => typD ts rs nil t
+			| None => unit
+		      end)
+	with
+  	  | Some t => fun pf => match pf in _ = t return
+  				      match t with
+                                        | Some T => projT1 T
+                                        | None => Empty_set
+                                      end with
+  				  | eq_refl => @lfalse _ (projT2 t)
+  				end
+  	  | None => fun _ => tt
+  	end eq_refl
+      | ilf_and i =>
+	match PositiveMap.find i ts as x
+	      return x = PositiveMap.find i ts ->
+		     (match match x with
+			      | Some _ => Some (tyArr (tyPred i) (tyArr (tyPred i) (tyPred i)))
+			      | None => None
+			    end
+		      with
+			| Some t => typD ts rs nil t
+			| None => unit
+		      end)
+	with
+  	  | Some t => fun pf => match pf in _ = t return
+  				      match t with
+                                        | Some T => projT1 T
+                                        | None => Empty_set
+                                      end ->
+                                      match t with
+                                        | Some T => projT1 T
+                                        | None => Empty_set
+                                      end ->
+                                      match t with
+                                        | Some T => projT1 T
+                                        | None => Empty_set
+                                      end
+                                with
+  				  | eq_refl => @land _ (projT2 t)
+  				end
+  	  | None => fun _ => tt
+  	end eq_refl
+      | ilf_or i =>
+	match PositiveMap.find i ts as x
+	      return x = PositiveMap.find i ts ->
+		     (match match x with
+			      | Some _ => Some (tyArr (tyPred i) (tyArr (tyPred i) (tyPred i)))
+			      | None => None
+			    end
+		      with
+			| Some t => typD ts rs nil t
+			| None => unit
+		      end)
+	with
+  	  | Some t => fun pf => match pf in _ = t return
+  				      match t with
+                                        | Some T => projT1 T
+                                        | None => Empty_set
+                                      end ->
+                                      match t with
+                                        | Some T => projT1 T
+                                        | None => Empty_set
+                                      end ->
+                                      match t with
+                                        | Some T => projT1 T
+                                        | None => Empty_set
+                                      end
+                                with
+  				  | eq_refl => @lor _ (projT2 t)
+  				end
+  	  | None => fun _ => tt
+  	end eq_refl
+      | ilf_impl i =>
+	match PositiveMap.find i ts as x
+	      return x = PositiveMap.find i ts ->
+		     (match match x with
+			      | Some _ => Some (tyArr (tyPred i) (tyArr (tyPred i) (tyPred i)))
+			      | None => None
+			    end
+		      with
+			| Some t => typD ts rs nil t
+			| None => unit
+		      end)
+	with
+  	  | Some t => fun pf => match pf in _ = t return
+  				      match t with
+                                        | Some T => projT1 T
+                                        | None => Empty_set
+                                      end ->
+                                      match t with
+                                        | Some T => projT1 T
+                                        | None => Empty_set
+                                      end ->
+                                      match t with
+                                        | Some T => projT1 T
+                                        | None => Empty_set
+                                      end
+                                with
+  				  | eq_refl => @limpl _ (projT2 t)
+  				end
+  	  | None => fun _ => tt
+  	end eq_refl
+      | fref fi => 
+        match PositiveMap.find fi fs as x
+              return match 
+                match x with
+                  | None => None
+                  | Some f0 => Some f0.(ftype)
+                end
+              with
+                | None => unit
+                | Some t => typD ts rs nil t
+              end
+        with
+          | None => tt
+          | Some f => f.(fdenote)
+        end
+    end.
+
+  Global Instance RFunc_ilfunc : RFunc (@typD ts rs) ilfunc :=
+  { typeof_func := typeof_func
+  ; funcD := funcD
+  }.
+End RFunc.
+
+
+Section demo.
+  Context {T : Type} {ILO : ILogicOps T}.
+
+  Definition logics : var_logic_map :=
+    PositiveMap.add 1%positive (@existT _ ILogicOps _ ILO) (PositiveMap.empty _).
+  Definition types : ref_type_map :=
+    PositiveMap.empty _.
+
+  Definition funcs : fun_map logics types := PositiveMap.empty _.
+
+  Definition tm : expr typ ilfunc :=
+    Inj (ilf_true 1%positive).
+
+  Require Import MirrorCore.Ext.ExprD.
+
+  (** TODO: Here we run into a problem because the [expr] type is
+   ** fixed to the [typ] defined in [MirrorCore.Ext.Types].
+   ** - To solve this problem, we need to abstract [expr] with respect to
+   **   types.
+   **)
+  Eval simpl in @exprD _ _ (RFunc_ilfunc _ _ _) nil nil tm (tyPred 1%positive).
+
+End demo.
